Comment code

StaticAnalyser.fst
@@ -1,31 +1,36 @@
+(*
+This module implements the core functions (leveraging AbstractDomain & GaloisConnection module's definitions) of a tiny WIP static analyser
+@summary: Toy static analyser's core
+*)
 module StaticAnalyser
 
 open FStar.GSet
 module CS = CSet
-open FStar.Tactics
 open FStar.Tactics.Typeclasses
 
-open PartialOrder
 open GaloisConnection
-open DefaultValue
 open ToyLanguageDef
 open EnumerableMap
 open AbstractDomain
 open ZeroOrLess
 
+(* Compute the (abstract) result of an expression *)
 let rec static_analysis_aexp #a [| hasGaloisConnection int a |] [| hasAbstractOperators a |]
                     (st:enumerableMap a)
                     (exp:lAExp)
                     : a
   = let rec h (exp:lAExp): a = 
          match exp with
-       | LAExpLitt n       -> alpha' n
-       | LAExpVar  varName -> em_get st varName
-       | LAExpPlus a b     -> (h a) `a_op_plus` (h b)
-       | LAExpMinus a b    -> (h a) `a_op_minus` (h b)
-       | LAExpMult a b    ->  (h a) `a_op_times` (h b)
+       | LAExpLitt  n       -> alpha' n
+       | LAExpVar   varName -> em_get st varName
+       | LAExpPlus  a b     -> (h a) `a_op_plus` (h b)
+       | LAExpMinus a b     -> (h a) `a_op_minus` (h b)
+       | LAExpMult  a b     ->  (h a) `a_op_times` (h b)
     in h exp
 
+(* Given an aim and an expression, the following function constraints 
+   the variable abstract values present in the expression, using generically
+   defined backward operators (see AbstractDomain module) *)
 let rec backward_analysis_aexp #a [| hasGaloisConnection int a |] [| hasAbstractOperators a |]
                                   [| hasAbstractDomain a |]
                     (st:enumerableMap a)
@@ -34,24 +39,29 @@ let rec backward_analysis_aexp #a [| hasGaloisConnection int a |] [| hasAbstract
                     : Tot (enumerableMap a) (decreases exp)
 = let f exp = static_analysis_aexp st exp in
   match exp with
-  | LAExpLitt n       -> st //(alpha' n) `inter` aim
-  | LAExpVar  varName -> em_set st varName aim//(st varName) ``
-  | LAExpPlus e1 e2   -> let (aim1, aim2):(tuple2 a a) = backward_aop_plus (f e1) (f e2) aim in (* e1 + e1 should fit in aim *)
+  | LAExpLitt n       -> st (* a constant cannot be refined *)
+  | LAExpVar  varName -> em_set st varName aim (* TODO: why do I set the value directly? should do some inter or smth *)
+  | LAExpPlus e1 e2   -> let (aim1, aim2):(tuple2 a a) = backward_aop_plus (f e1) (f e2) aim in (* e1 + e2 should fit in aim *)
                         let st' = backward_analysis_aexp st e1 aim1 in
                         backward_analysis_aexp st' e2 aim2
-  | LAExpMinus e1 e2  -> let (aim1, aim2):(tuple2 a a) = backward_aop_minus (f e1) (f e2) aim in (* e1 + e1 should fit in aim *)
+  | LAExpMinus e1 e2  -> let (aim1, aim2):(tuple2 a a) = backward_aop_minus (f e1) (f e2) aim in (* e1 - e1 should fit in aim *)
                         let st' = backward_analysis_aexp st e1 aim1 in
                         backward_analysis_aexp st' e2 aim2
   | LAExpMult a b    ->  st (*todo*)//(h a) `a_op_times` (h b)
 
+(* Given an boolean expression `bexp` and a state, `analyse_bexp` returns a state satisfying `bexp` *)
 let rec analyse_bexp #a [| hasAbstractOperators a |] [| hasAbstractDomain a |] [| hasGaloisConnection int a |] [| hasZeroOrLess a |]
                      (st:enumerableMap a)
                      (exp:lBExp): Tot (enumerableMap a)
+                                  (* either the number of non-terminal `not` is decreasing, either
+                                     the size of exp (i.e. the deepness of the AST) is decreasing *)
                                   (decreases %[bexp_count_not exp; exp])
   = match exp with
   | LBExpLitt b -> if b then st (* supposing true doesn't bring anything new *)
                        else {_em_data = (fun _ -> bottom); _em_keys = st._em_keys} (* variables should all be bottom *)
+  (* if `not` is terminal (i.e. `! (3 <= 45)`) *)
   | LBExpNot (LBExpEq a b) -> backward_analysis_aexp st (a -. b) (alpha' 0)
+  (* otherwise, we apply demorgan and `a <= b ==> b <= a && !(a==b)` *)
   | LBExpNot  b -> let rec apply_not (e:lBExp): (r:lBExp{bexp_count_not e >= bexp_count_not r}) = (match e with
                           | LBExpNot e1    -> e1
                           | LBExpAnd e1 e2 -> LBExpOr  (apply_not e1) (apply_not e2)
@@ -62,11 +72,14 @@ let rec analyse_bexp #a [| hasAbstractOperators a |] [| hasAbstractDomain a |] [
                           ) in 
                             let nexp = apply_not b in
                                analyse_bexp st nexp
+                     (* `em_combine` takes two states and apply a function for 
+                        each pairs of values that share a same key *)
   | LBExpAnd  a b -> em_combine (analyse_bexp st a) (analyse_bexp st b) inter
   | LBExpOr   a b -> em_combine (analyse_bexp st a) (analyse_bexp st b) union
   | LBExpEq   a b -> backward_analysis_aexp st (a -. b) (alpha' 0)//lessThanZero
   | LBExpLe   a b -> backward_analysis_aexp st (a -. b) zeroOrLess
 
+(* This functions perform static analysis on instructions, i.e. on full programs *)
 let rec static_analysis_instr #a [| hasAbstractOperators a |] [| hasAbstractDomain a |] [| hasGaloisConnection int a |] [| hasZeroOrLess a |]
                     (st:enumerableMap a)
                     (instr:lInstr)
@@ -79,10 +92,14 @@ let rec static_analysis_instr #a [| hasAbstractOperators a |] [| hasAbstractDoma
   | LInstrIf c b1 b2    -> let r1 = f (analyse_bexp st     c ) b1 in
                           let r2 = f (analyse_bexp st (!. c)) b2 in
                           em_combine r1 r2 union
-  | LInstrWhile cond b1 -> let apply_cond st = analyse_bexp st cond in
+  | LInstrWhile cond b1 -> let apply_cond st = analyse_bexp st cond in 
+                          (* apply_cond takes a state: at each iterations, inveriants 
+                             might change, so we need to recompute the condition *)
+                          (* TODO: remove that stop parameter *)
                           let rec lookForFixPoint current_st (stop: nat): Tot (enumerableMap a) = if stop=0 then current_st else
-                              let new_st  = static_analysis_instr (apply_cond current_st) b1 in
-                              let widened = em_combine new_st (apply_cond (em_combine current_st new_st widen)) union in 
-                                if   em_equal aeq current_st widened then widened
-                                else lookForFixPoint (admitP (%[widened] << %[current_st]); widened) (stop - 1) in
+                              let new_st  = static_analysis_instr (apply_cond current_st) b1 in (* compute while's body once *)
+                              let widened = em_combine new_st (apply_cond (em_combine current_st new_st widen)) union in (* widen the new state *)
+                                if   em_equal aeq current_st widened then widened (* we reached a fixpoint, we're done *)
+                                else lookForFixPoint (admitP (%[widened] << %[current_st]); widened) (stop - 1) in (* TODO: prove some lemma saying widening is ensures termination *)
+                          (* we combine the fixpoint state with the old state constrained with the negated condition *)
                           em_combine (analyse_bexp st (!. cond)) (lookForFixPoint st 4) union
