ToString.fst
@@ -1,10 +1,19 @@
+(*
+@summary: a -> string interface
+*)
 module ToString
 
 open FStar.Tactics.Typeclasses
 open FStar.String
+open FStar.List.Tot.Base
 
 class hasToString t = {
   toString: t -> string
 }
 
-let join sep l = List.Tot.Base.fold_right (fun a b -> (if a = "" then sep else "") `strcat` (a `strcat` b)) l ""
+let join sep l = fold_right
+					(fun (a, i) b -> (if i then sep else "") `strcat` (a `strcat` b))
+					(mapi (fun i x -> (x, i > 0)) l)
+					""
+private
+let example = join "," ["A";"B";"C";"D"]
